Working on fixing the animations

Animate.lean
@@ -1,86 +1,568 @@
 import Lean
-import Batteries
+import Lean.Data.Json.FromToJson
 import Mathlib.Tactic
-import Lean.Elab
+
+import Annotations
+import HighlightSyntax
+import StringMatching
+
+namespace Animate
+
+--- animate.lean command line arguments
+structure Config where
+  file_path : System.FilePath := "."
+  const_name : Lean.Name := `Unknown
+  print_infotree : Bool := true
+  print_stage1 : Bool := true
+  print_stage2 : Bool := true
+  min_match_len : Nat := 2
+  nonmatchers : String := ""
+
+def parseArgs (args : Array String) : IO Config := do
+  if args.size < 2 then
+    throw <| IO.userError "usage: animate FILE_PATH CONST_NAME"
+  let mut cfg : Config := {}
+  cfg := { cfg with file_path := ⟨args[0]!⟩ }
+  cfg := { cfg with const_name := args[1]!.toName }
+  let mut idx := 2
+  while idx < args.size do
+    match args[idx]! with
+    | "--print-infotree" =>
+       cfg := {cfg with print_infotree := true}
+    | "--print-stage1" =>
+       cfg := {cfg with print_stage1 := true}
+    | "--print-stage2" =>
+       cfg := {cfg with print_stage2 := true}
+    | "--min-match-len" =>
+       idx := idx + 1
+       let x := args[idx]!.toNat!
+       cfg := {cfg with min_match_len := x}
+    | "--nonmatchers" =>
+       idx := idx + 1
+       let x := args[idx]!
+       cfg := {cfg with nonmatchers := x}
+    | s => throw <| IO.userError s!"unknown argument {s}"
+    idx := idx + 1
+
+  return cfg
+
+--------------------------------------------------
+
+-- json that we send to animate.py for blender rendering
+
+structure Goal where
+  --- MVarId
+  goalId : String
+  state : String
+deriving Lean.ToJson, Lean.FromJson, BEq
+
+structure TransformedGoal where
+  goal : Goal
+  indexMaps : IndexMaps
+deriving Lean.ToJson, Lean.FromJson
+
+structure GoalAction where
+  --- MVarId from before the tactic is applied.
+  startGoalId : String
+
+  --- Pretty-printed goal state before the tactic is applied.
+  startState : String
+
+  -- empty means the goal has been closed.
+  results : List TransformedGoal
+deriving Lean.ToJson, Lean.FromJson
+
+--- Application of a single tactic.
+--- It may act on multiple goals (e.g. when using the <;> combinator).
+structure Action where
+  tacticText : String
+  goalActions : List GoalAction
+deriving Lean.ToJson, Lean.FromJson
+
+structure GoalHighlighting where
+  goalId : String
+  colors : HighlightSyntax.ColorMap
+deriving Lean.ToJson, Lean.FromJson
+
+-- Result of stage 3.
+-- To be jsonified and consumed by animate.py in Blender
+structure Movie where
+  theoremName : String
+  startGoal : Goal
+  actions: List Action
+  highlighting: Array GoalHighlighting
+deriving Lean.ToJson, Lean.FromJson
+
+------------------
+
+-- intermediate representation
+-- stage 1: tree of tactic sequences
+
+instance : Lean.ToJson String.Pos where
+  toJson := fun p ↦ Lean.Json.num p.byteIdx
+
+instance : Lean.FromJson String.Pos where
+    fromJson? := fun j ↦ do
+  let idx ← j.getNat?
+  return ⟨idx⟩
+
+structure StringSpan where
+  startPos : String.Pos
+  endPos : String.Pos
+deriving Lean.ToJson, Lean.FromJson, BEq
+
+structure TacticStepData where
+  elaborator : String
+  name : String
+
+  --- The text of the tactic, with any child tactic
+  --- text replaced by "?_"
+  text : String
+
+  tacticSpan : StringSpan
+  goals_before : List Goal
+  goals_after : List Goal
+  reverse_s1 : Bool := false
+  reverse_s2 : Bool := false
+deriving Lean.ToJson, Lean.FromJson
+
+structure SeqData where
+  tacticSpan : StringSpan
+  goals_before : List Goal
+  goals_after : List Goal
+deriving Lean.ToJson, Lean.FromJson
+
+inductive TacticStep where
+| node (data : TacticStepData)
+       (children : List TacticStep)
+| seq (span: StringSpan) (children : List TacticStep)
+deriving Lean.ToJson, Lean.FromJson
+
+def TacticStep.goals_before : TacticStep →  List Goal
+| .node data _ => data.goals_before
+| .seq _ [] => []
+| .seq _ (c::_) => c.goals_before
+
+--------------------
+-- stage 2: flattened map of tactic steps.
+
+structure TacticStep' where
+  text : String
+  span : StringSpan
+  goal_before : Goal
+  goals_after : List Goal -- include children
+  reverse_s1 : Bool := false
+  reverse_s2 : Bool := false
+deriving Lean.ToJson, Lean.FromJson
+
+/-- map from goalId to tactic step that consumes that goal.
+    That should be the latest, most specific step
+    that lists the goal in its before state but not in its after state.
+-/
+abbrev StepMap := Std.HashMap String TacticStep'
+
+structure Stage2State where
+  startGoal : Goal
+  steps : StepMap
+
+def Stage2State.dump (s : Stage2State) : IO Unit := do
+  IO.println <| "stage2 with top goal " ++ s.startGoal.goalId
+  for ⟨_, ts⟩ in s.steps.toList do
+    IO.println <| s!"{Lean.ToJson.toJson ts}"
+  -- TODO
+
+section syntax_manip
 
 open Lean
+
+def StringSpan.ofSyntax (stx : Syntax) : Option StringSpan := Id.run do
+  let some p1 := stx.getPos? | return none
+  let some p2 := stx.getTailPos? | return none
+  return .some ⟨p1, p2⟩
+
+def replace_inner_syntax (src : String) (outer : StringSpan) (inners : List StringSpan)
+    (replacement : String := "?_") :
+    String := Id.run do
+  let mut result := ""
+  let mut curPos := outer.startPos
+  for inner in inners do
+    result := result ++
+      (Substring.mk src curPos inner.startPos).toString ++ replacement
+    curPos := inner.endPos
+  result := result ++ (Substring.mk src curPos outer.endPos).toString
+  return result
+
+--#eval replace_inner_syntax
+--       "have h := by rfl" ⟨⟨0⟩, ⟨17⟩⟩ [⟨⟨13⟩, ⟨17⟩⟩]
+
+def left_trim_lines (lines : String) (col : Nat) : String := Id.run do
+  let mut lines := lines.splitOn "\n"
+  let mut rev_result := []
+  for line in lines do
+    let pfx := Substring.mk line ⟨0⟩ ⟨col⟩
+    if pfx.toString = String.replicate col ' '
+    then rev_result := line.drop col :: rev_result
+    else rev_result := line :: rev_result
+  return String.intercalate "\n" rev_result.reverse
+
+-- #eval left_trim_lines "a\n  bc\n   d" 2
+
+def StringSpan.union (s1 s2 : StringSpan) : StringSpan :=
+  { startPos := ⟨min s1.startPos.byteIdx s2.startPos.byteIdx⟩,
+    endPos := ⟨max s1.endPos.byteIdx s2.endPos.byteIdx⟩,
+  }
+
+def EMPTY_SPAN : StringSpan := {startPos := ⟨0xffffffffffffffff⟩, endPos := ⟨0⟩}
+
+def StringSpan.union_list : List StringSpan → StringSpan
+| [] => EMPTY_SPAN
+| s :: ss => s.union (StringSpan.union_list ss)
+
+unsafe def TacticStep.span_union : TacticStep → StringSpan
+| .node data children =>
+     let children_spans := children.map (fun c ↦ c.span_union)
+     data.tacticSpan.union (StringSpan.union_list children_spans)
+| .seq span children =>
+     span.union (StringSpan.union_list (children.map (fun c ↦ c.span_union)))
+
+
+end syntax_manip
+
+section infotrees
+
 open Lean Elab
 
+def collectNodesBottomUpM {α : Type} {m : Type → Type} [Monad m]
+    (p : ContextInfo → Info → PersistentArray InfoTree → List α → m (List α))
+    (i : InfoTree) : m (List α) := do
+  let x ← i.visitM
+   (m := m)
+   (postNode := fun ci i cs as => p ci i cs (as.filterMap id).flatten)
+  let y := x.getD []
+  return y
 
-#eval 1 + 2
+/-- Find the name for the outermost `Syntax` in this `TacticInfo`. -/
+def _root_.Lean.Elab.TacticInfo.name? (t : TacticInfo) : Option Name :=
+  match t.stx with
+  | Syntax.node _ n _ => some n
+  | _ => none
 
-def main : IO Unit := do
-  IO.println "Hello, Lean!"
+def GOAL_PP_WIDTH : Nat := 80
 
-unsafe def processCommands : Frontend.FrontendM (List (Environment × InfoState)) := do  -- define a function to process commands in the frontend monad
-  let done ← Lean.Elab.Frontend.processCommand  -- process the command getting the parser state, command, and the command state and the input context
-  let st := ← get -- get the current state of the frontend
-  let infoState := st.commandState.infoState  -- get the info state from the command state
-  let env' := st.commandState.env -- get the environment from the command state
+unsafe def visitTacticInfo (ci : ContextInfo) (ti : TacticInfo)
+    (acc : List TacticStep) : IO (List TacticStep) := do
+  let src := ci.fileMap.source
+  let stx := ti.stx
+
+  let .some startPos := stx.getPos? | return acc
+  let startPosition := ci.fileMap.toPosition startPos
+  let .some span := StringSpan.ofSyntax stx | return acc
+
+  let mut goals_before := []
+  for g in ti.goalsBefore do
+    let doprint : MetaM _ := Meta.ppGoal g
+    let cm := doprint.run' (s := { mctx := ti.mctxBefore })
+    let fm ← ci.runCoreM cm
+    goals_before := goals_before ++ [⟨g.name.toString, fm.pretty (width := GOAL_PP_WIDTH)⟩]
+
+    let _x := ti.mctxAfter.getExprAssignmentCore? g
+    -- collect all fvars that appear in x ...
+    --
+    --dbg_trace x
+
+  let mut goals_after := []
+  for g in ti.goalsAfter do
+    let doprint : MetaM _ := Meta.ppGoal g
+    let cm := doprint.run' (s := { mctx := ti.mctxAfter })
+    let fm ← ci.runCoreM cm
+    goals_after := goals_after ++ [⟨g.name.toString, fm.pretty (width := GOAL_PP_WIDTH)⟩]
+
+  if let some ``Lean.Parser.Tactic.tacticSeq1Indented := ti.name?
+  then
+    if acc.length > 0 then
+    return [TacticStep.seq EMPTY_SPAN acc]
+
+  if let .atom _ "by" := ti.stx then
+    if acc.length > 0 then
+      return [TacticStep.seq span acc]
+    else return acc
+
+  match stx.getHeadInfo? with
+  | .some (.synthetic ..) =>
+    -- Not actual concrete syntax the user wrote. Ignore.
+    return acc
+  | _ => pure ()
+
+  -- Tactic step is a no-op. Ignore it.
+  if goals_before == goals_after then return acc
+
+  let .some name := ti.name? | return acc
+  match name with
+  | `null => return acc
+--  | ``Lean.Parser.Term.byTactic =>
+--      return [TacticStep.seq ⟨span, goals_before, goals_after⟩ acc]
+  | ``cdotTk => return acc
+  | ``atomicTac =>
+     if let .node _ ``atomicTac #[_, _, inner, _] := ti.stx then
+       let .some span' := StringSpan.ofSyntax inner | panic! "bad atomic span"
+       let .some startPos := inner.getPos? | panic! "bad inner span"
+       let startPosition := ci.fileMap.toPosition startPos
+       let text := replace_inner_syntax src span' []
+       let text := left_trim_lines text startPosition.column
+
+       let d := { elaborator := ti.elaborator.toString
+                  name := name.toString
+                  tacticSpan := span'
+                  text
+                  goals_before, goals_after }
+       return [TacticStep.node d []]
+     else
+       panic! "bad atomic syntax"
+  | ``reverseS2Tac =>
+     if let .node _ ``reverseS2Tac #[_, _, inner, _] := ti.stx then
+       let .some span' := StringSpan.ofSyntax inner | panic! "bad reverse_s2 span"
+       let .some startPos := inner.getPos? | panic! "bad inner span"
+       let startPosition := ci.fileMap.toPosition startPos
+       let text := replace_inner_syntax src span' []
+       let text := left_trim_lines text startPosition.column
+
+       let d := { elaborator := ti.elaborator.toString
+                  name := name.toString
+                  tacticSpan := span'
+                  text
+                  reverse_s2 := true
+                  goals_before, goals_after }
+       return [TacticStep.node d []]
+     else
+       panic! "bad reverse_s2 syntax"
+
+  | ``reverseS1S2Tac =>
+     if let .node _ ``reverseS1S2Tac #[_, _, inner, _] := ti.stx then
+       let .some span' := StringSpan.ofSyntax inner | panic! "bad reverse_s1_s2 span"
+       let .some startPos := inner.getPos? | panic! "bad inner span"
+       let startPosition := ci.fileMap.toPosition startPos
+       let text := replace_inner_syntax src span' []
+       let text := left_trim_lines text startPosition.column
+
+       let d := { elaborator := ti.elaborator.toString
+                  name := name.toString
+                  tacticSpan := span'
+                  text
+                  reverse_s1 := true
+                  reverse_s2 := true
+                  goals_before, goals_after }
+       return [TacticStep.node d []]
+     else
+       panic! "bad reverse_s1_s2 syntax"
+
+
+  | ``reverseS1Tac =>
+     if let .node _ ``reverseS1Tac #[_, _, inner, _] := ti.stx then
+       let .some span' := StringSpan.ofSyntax inner | panic! "bad reverse_s1 span"
+       let .some startPos := inner.getPos? | panic! "bad inner span"
+       let startPosition := ci.fileMap.toPosition startPos
+       let text := replace_inner_syntax src span' []
+       let text := left_trim_lines text startPosition.column
+
+       let d := { elaborator := ti.elaborator.toString
+                  name := name.toString
+                  tacticSpan := span'
+                  text
+                  reverse_s1 := true
+                  goals_before, goals_after }
+       return [TacticStep.node d []]
+     else
+       panic! "bad reverse_s1 syntax"
+
+
+  | ``Lean.Parser.Tactic.inductionAlt =>
+    -- induction alternative. We want the direct children
+    -- of `induction` to be `seq` nodes, so we collapse these.
+    return acc
+  | _ => pure ()
+
+  let mut inners := []
+  for c in acc do
+    inners := inners ++ [c.span_union]
+
+  let text := replace_inner_syntax src span inners
+  let text := left_trim_lines text startPosition.column
+
+  let d := { elaborator := ti.elaborator.toString
+             name := name.toString
+             tacticSpan := span
+             text
+             goals_before, goals_after }
+  return [TacticStep.node d acc]
+
+unsafe def visitNode (ci : ContextInfo) (info : Info)
+    (_children : PersistentArray InfoTree)
+    (acc : List TacticStep) : IO (List TacticStep) :=
+  match info with
+  | .ofTacticInfo ti => visitTacticInfo ci ti acc
+  | _ => pure acc
+
+unsafe def extractToplevelStep (tree : InfoTree) : IO TacticStep := do
+  let steps ← collectNodesBottomUpM (m := IO) visitNode tree
+  let [step] := steps | throw <| IO.userError "got more than one toplevel step"
+  return step
+
+partial def stage2_aux (step : TacticStep) : StateM StepMap Unit := match step with
+| .node data children => do
+  if let [goal] := data.goals_before then
+    let sm ← get
+    let goalId := goal.goalId
+    let span := data.tacticSpan
+    -- goals after includes stuff from the children in addition to data.goals_after.
+    let mut goals_after := []
+    for child in children do
+      for g in child.goals_before do
+        goals_after := g :: goals_after
+    for g in data.goals_after do
+       goals_after := g :: goals_after
+    let ts' := { span,
+                 goal_before := goal,
+                 goals_after := goals_after.reverse,
+                 text := data.text,
+                 reverse_s1 := data.reverse_s1
+                 reverse_s2 := data.reverse_s2 }
+    set (sm.insert goalId ts')
+  for child in children do
+    stage2_aux child
+| .seq _ children => do
+  for child in children do
+    stage2_aux child
+
+partial def stage2 (step : TacticStep) : IO Stage2State := do
+  let ⟨_, m⟩ := StateT.run (stage2_aux step) default
+  let [top_goal] := step.goals_before |
+         throw <| IO.userError "got more than one toplevel step"
+  return { startGoal := top_goal, steps := m }
+
+
+def stage3_inner (config : Config) (step : TacticStep') : GoalAction := Id.run do
+    let mut ts_rev : List TransformedGoal := []
+    for g in step.goals_after do
+      let im := Animate.do_match step.goal_before.state g.state
+                                 (min_match_len := config.min_match_len)
+                                 (nonmatchers := config.nonmatchers)
+                                 (s1_reverse_order := step.reverse_s1)
+                                 (s2_reverse_order := step.reverse_s2)
+      ts_rev := {goal := g, indexMaps := im} :: ts_rev
+    let ga : GoalAction := {
+      startGoalId := step.goal_before.goalId
+      startState := step.goal_before.state
+      results := ts_rev.reverse
+    }
+    return ga
+
+partial def stage3 (config : Config) (state2 : Stage2State) : IO Movie := do
+  let mut rev_actions := []
+  let mut visited := Batteries.mkRBSet String Ord.compare
+  let mut colorings := #[]
+  let mut currentGoals := [state2.startGoal.goalId]
+  while currentGoals.length > 0 do
+    let currentGoal :: rest := currentGoals | panic "impossible"
+    if visited.contains currentGoal then panic s!"re-visited goal {currentGoal}"
+    visited := visited.insert currentGoal
+    let .some step :=
+      state2.steps.get? currentGoal | panic s!"goal not found {currentGoal}"
+    colorings := colorings.push ⟨currentGoal, ← HighlightSyntax.assign_colors step.goal_before.state⟩
+    let mut goal_actions := [stage3_inner config step]
+    currentGoals := []
+    for gid in rest do
+      let .some other_step :=
+        state2.steps.get? gid | panic s!"goal not found {gid}"
+      if other_step.span == step.span
+      then
+        colorings := colorings.push ⟨gid, ← HighlightSyntax.assign_colors other_step.goal_before.state⟩
+        goal_actions := stage3_inner config other_step :: goal_actions
+        currentGoals := currentGoals ++ (other_step.goals_after.map (·.goalId))
+      else
+        currentGoals := currentGoals ++ [gid]
+
+    rev_actions := { tacticText := step.text, goalActions := goal_actions } :: rev_actions
+    currentGoals := (step.goals_after.map (·.goalId)) ++ currentGoals
+    pure ()
+  -- TODO: verify that everything in state2 was visited.
+  return { theoremName := config.const_name.toString
+           actions := rev_actions.reverse
+           startGoal := state2.startGoal,
+           highlighting := colorings}
+
+unsafe def processCommands : Frontend.FrontendM (List (Environment × InfoState)) := do
+  let done ← Lean.Elab.Frontend.processCommand
+  let st := ← get
+  let infoState := st.commandState.infoState
+  let env' := st.commandState.env
 
   -- clear the infostate
-  set {st with commandState := {st.commandState with infoState := {}}}  -- clear the info state
+  set {st with commandState := {st.commandState with infoState := {}}}
   if done
   then return [(env', infoState)]
   else
-    return (env', infoState) :: (←processCommands)  -- recursively call the processCommands function until done is true
+    return (env', infoState) :: (←processCommands)
 
-unsafe def processFile (filePath : String) : IO Unit := do
-  let mut input ← IO.FS.readFile filePath -- reads the contents of the file
-  let inputCtx := Lean.Parser.mkInputContext filePath input -- takes in the file data and the file path to be parsed
-  let (header, parserState, messages) ← Lean.Parser.parseHeader inputCtx  -- parses the header
-  let (env, messages) ← Lean.Elab.processHeader header {} messages inputCtx -- processes the header and creates the environment
+unsafe def processFile (config : Config) : IO Unit := do
+  IO.println "Flag 1"
+  Lean.searchPathRef.set compile_time_search_path%
+  IO.println "Flag 2"
+  let mut input ← IO.FS.readFile config.file_path
+  IO.println "Flag 3"
+  Lean.enableInitializersExecution
+  IO.println "Flag 4"
+  let inputCtx := Lean.Parser.mkInputContext input config.file_path.toString
+  IO.println "Flag 5"
+  let (header, parserState, messages) ← Lean.Parser.parseHeader inputCtx
+  IO.println "Flag 6"
+  let (env, messages) ← Lean.Elab.processHeader header {} messages inputCtx
+  IO.println "Flag 7"
 
-  IO.println s!"{filePath}"
+  if messages.hasErrors then
+    for msg in messages.toList do
+      if msg.severity == .error then
+        println! "ERROR: {← msg.toString}"
+    throw <| IO.userError "Errors during import; aborting"
 
-  let env := env.setMainModule (← Lean.moduleNameOfFileName filePath none)  -- sets the main module to the file name
+  let env := env.setMainModule (← Lean.moduleNameOfFileName config.file_path none)
 
-  let commandState := { Lean.Elab.Command.mkState env messages {} with infoState.enabled := true }  -- creates the command state with the environment and messages
 
-  let (steps, _frontendState) ← (processCommands { inputCtx := inputCtx }).run  -- runs the processCommands function with the input context and command state
-    { commandState := commandState, parserState := parserState, cmdPos := parserState.pos } -- sets the command state and parser state
+  if env.contains config.const_name then
+    throw <| IO.userError s!"constant of name {config.const_name} is already in environment"
 
-  -- output all of the before and after states of the info tree
-  IO.println s!"{steps.length} steps"
+  let commandState := { Lean.Elab.Command.mkState env messages {} with infoState.enabled := true }
+
+  let (steps, _frontendState) ← (processCommands.run { inputCtx := inputCtx }).run
+    { commandState := commandState, parserState := parserState, cmdPos := parserState.pos }
+
+  -----
   for ⟨env, s⟩ in steps do
-    IO.println s!"{s.infoState}"
-    -- get the info tree from the info state
-    let infoTree := s.infoState.infoTree
+    if env.contains config.const_name then
+      for tree in s.trees do
+        if config.print_infotree then
+           IO.println (Format.pretty (←tree.format))
+        let step ← extractToplevelStep tree
+        if config.print_stage1 then
+          IO.println s!"{ToJson.toJson step}"
+        let stage2state ← stage2 step
+        if config.print_stage1 then
+          IO.println "STAGE 2:"
+          stage2state.dump
+        let stage3 ← stage3 config stage2state
+        IO.println <| (Lean.toJson stage3).pretty (lineWidth := 200)
+      -- we're done
+      return ()
 
-  for ⟨env, s⟩ in steps do
-    for tree in s.trees do
-      IO.println (Format.pretty (←tree.format))
-      let flattened := tree.context
-      for ⟨goal _⟩ in flattened do
-        IO.println (Format.pretty (←goal.format))
+  throw <| IO.userError s!"no constant of name {config.const_name} was found"
 
-  throw <| IO.userError s!"{steps.length} steps"
+end infotrees
 
+end Animate
 
+unsafe def main (args : List String) : IO Unit := do
+  IO.println "Flag -1"
+  let cfg ← Animate.parseArgs args.toArray
 
--- #eval processFile "AnimateProofs/Test.lean"
+  IO.println "Flag 0"
 
-
-/-
--- read the infotree of a given file
-open Lean
-open System
-
-def readInfoTree (filePath : String) : IO Unit := do
-  let env ← importModules [{ module := `Init }] {}
-  let input ← IO.FS.readFile filePath
-  let (_, infoTree) ← Lean.Elab.Command.elabCommand input env
-  IO.println infoTree
-
--- Example usage
-#eval readInfoTree "C:\Users\lukec\OneDrive\Documents\AnimateProofs\AnimateProofs\Test.lean"
--/
-
-/-
-set_option trace.Elab.info true
-example : 2 = 1 + 1 := by
-  show 1 + 1 = 2
-  rw[one_add_one_eq_two]
-
-set_option trace.Elab.info false
--/
+  Animate.processFile cfg
