HighlightSyntax.lean
@@ -1,0 +1,122 @@
+import Lean
+import Std.Internal.Parsec
+
+namespace HighlightSyntax
+
+/-- For each character index in the text, a
+    Nat represting the color at that index.
+-/
+abbrev ColorMap := Array Nat
+
+
+def cat_to_color : String → Nat
+| "Token.Text" => 1
+| "Token.Text.Whitespace" => 2
+| "Token.Keyword" => 3
+| "Token.Name" => 4
+| "Token.Name.Builtin.Pseudo" => 5
+| "Token.Operator" => 6
+| "Token.Literal.Number.Integer" => 7
+| _ => 0
+
+
+section parse
+
+/-
+This section is a lightly adapted copy of some stuff from Lean/Data/Json/Parser.lean.
+-/
+
+open Lean
+
+namespace Parse
+
+def hexChar : Std.Internal.Parsec String.Iterator Nat := do
+  let c ← Std.Internal.Parsec.any
+  if '0' ≤ c ∧ c ≤ '9' then
+    pure $ c.val.toNat - '0'.val.toNat
+  else if 'a' ≤ c ∧ c ≤ 'f' then
+    pure $ c.val.toNat - 'a'.val.toNat + 10
+  else if 'A' ≤ c ∧ c ≤ 'F' then
+    pure $ c.val.toNat - 'A'.val.toNat + 10
+  else
+    Std.Internal.Parsec.fail "invalid hex character"
+
+def escapedChar : Std.Internal.Parsec String.Iterator Char := do
+  let c ← Std.Internal.Parsec.any
+  match c with
+  | '\\' => return '\\'
+  | '"'  => return '"'
+  | '/'  => return '/'
+  | 'b'  => return '\x08'
+  | 'f'  => return '\x0c'
+  | 'n'  => return '\n'
+  | 'r'  => return '\x0d'
+  | 't'  => return '\t'
+  | 'u'  =>
+    let u1 ← hexChar; let u2 ← hexChar; let u3 ← hexChar; let u4 ← hexChar
+    return Char.ofNat $ 4096*u1 + 256*u2 + 16*u3 + u4
+  | 'x'  =>
+    let b1 ← hexChar; let b2 ← hexChar
+    return Char.ofNat $ 16*b1 + b2
+
+  | _ => Std.Internal.Parsec.fail "illegal \\u escape"
+
+partial def strCore (acc : String) : Std.Internal.Parsec String.Iterator String := do
+  let c ← Std.Internal.Parsec.peek!
+  if c = '"' then -- "
+    Std.Internal.Parsec.skip
+    return acc
+  else
+    let c ← Std.Internal.Parsec.any
+    if c = '\\' then
+      strCore (acc.push (← escapedChar))
+    -- as to whether c.val > 0xffff should be split up and encoded with multiple \u,
+    -- the JSON standard is not definite: both directly printing the character
+    -- and encoding it with multiple \u is allowed. we choose the former.
+    else if 0x0020 ≤ c.val ∧ c.val ≤ 0x10ffff then
+      strCore (acc.push c)
+    else
+      Std.Internal.Parsec.fail "unexpected character in string"
+
+def str : Std.Internal.Parsec String.Iterator String := strCore ""
+
+end Parse
+end parse
+
+def assign_colors (s : String) : IO ColorMap := do
+  -- TODO randomize? or use stdio
+  let filename := "/tmp/animate-lean.txt"
+
+  IO.FS.writeFile filename s
+  let child ← IO.Process.spawn {
+    cmd := "pygmentize"
+    args := #["-l", "lean4", "-f", "raw", filename]
+    stdout := .piped
+  }
+
+  let output ← child.stdout.readToEnd
+  let exitCode ← child.wait
+  if exitCode != 0
+  then throw (IO.userError "pygmentize failed")
+
+  let mut result := #[]
+  let mut idx := 0
+  for line in output.split (· = '\n') do
+    if line = "" then continue
+    let [cat, val] := line.split (· = '\t') |
+      throw (IO.userError s!"bad pygmentize output: {line}")
+    let val' := (val.drop 1).dropRight 1 ++ "\""
+    match Parse.str val'.mkIterator with
+    | Std.Internal.Parsec.ParseResult.success _ v =>
+      for _c in v.toList do
+        result := result.push (cat_to_color cat)
+        idx := idx + 1
+
+    | Std.Internal.Parsec.ParseResult.error _ err  =>
+      throw (IO.userError s!"failed to parse string {val}: {err}")
+
+  let _ := s.length
+  --dbg_trace "lengths : {s.length} vs {result.size}"
+
+  --dbg_trace result
+  return result
