StringMatching.lean
@@ -1,0 +1,87 @@
+import Lean.Data.Json.FromToJson
+import Batteries.Data.List
+
+namespace Animate
+
+structure IndexMaps where
+  s1_to_s2 : Array (Option Nat)
+  s2_to_s1 : Array (Option Nat)
+deriving Lean.ToJson, Lean.FromJson
+
+structure BestMatch where
+  start_ii : Nat
+  start_jj : Nat
+  length : Nat
+
+def get_hyps_start (s1 : List Char) : Nat :=
+  match (s1.findIdx? (· = '\n'), s1.findIdx? (· = ':')) with
+  | (none, none) => 0
+  | (none, some _) => 0
+  | (some n, none) => n + 1
+  | (some nn, some nc) =>
+      if nn < nc then nn + 1 else 0
+
+def get_next_best_match (s1 s2 : List Char) (im : IndexMaps) (nonmatchers : String := "")
+    (s1_reverse_order := false)
+    (s2_reverse_order := false)
+    : BestMatch := Id.run do
+  let mut best : BestMatch := ⟨0, 0, 0⟩
+
+  -- HACK
+  let s1_hyps_start := get_hyps_start s1
+  let s2_hyps_start := get_hyps_start s2
+
+  let s1 := s1.toArray
+  let s2 := s2.toArray
+
+  let s1range := if s1_reverse_order then (List.range s1.size).reverse else List.range s1.size
+  let s2range := if s2_reverse_order then (List.range s2.size).reverse else List.range s2.size
+
+  for ii in s1range do
+    for jj in s2range do
+      let mut kk := 0
+      if s1.get! (ii + kk) ∉ nonmatchers.toList then
+      while ii + kk < s1.size && jj + kk < s2.size &&
+            s1.get! (ii + kk) = s2.get! (jj + kk) &&
+            im.s1_to_s2.get! (ii + kk) = none &&
+            im.s2_to_s1.get! (jj + kk) = none do
+        kk := kk + 1
+
+      if ii < s1_hyps_start ∧ s2_hyps_start ≤ jj
+      then continue
+
+      if s1_hyps_start ≤ ii ∧ jj < s2_hyps_start
+      then continue
+
+      if kk > best.length then
+        best := ⟨ii, jj, kk⟩
+  return best
+
+def do_match (s1 s2 : String) (min_match_len : Nat := 1) (nonmatchers : String := "")
+    (s1_reverse_order := false)
+    (s2_reverse_order := false)
+    : IndexMaps := Id.run do
+  let mut result := ⟨Array.mkArray s1.length none, Array.mkArray s2.length none⟩
+
+  let cs1 := s1.toList
+  let cs2 := s2.toList
+
+  -- HACK : don't let the ⊢ combine with stuff around it.
+  if let ⟨some idx1, some idx2⟩ := (cs1.findIdx? (· = '⊢'), cs2.findIdx? (· = '⊢')) then
+    result :=
+      ⟨result.s1_to_s2.set! idx1 (some idx2),
+       result.s2_to_s1.set! idx2 (some idx1)⟩
+    pure ()
+
+  while True do
+    let m := get_next_best_match cs1 cs2 result (nonmatchers := nonmatchers)
+               (s1_reverse_order := s1_reverse_order)
+               (s2_reverse_order := s2_reverse_order)
+    if m.length < min_match_len then
+      return result
+    for kk in [0 : m.length] do
+      result :=
+        ⟨result.s1_to_s2.set! (m.start_ii + kk) (some (m.start_jj + kk)),
+         result.s2_to_s1.set! (m.start_jj + kk) (some (m.start_ii + kk))⟩
+    pure ()
+  return result
